elo-coq/Map.v
@@ -1,179 +1,65 @@
 From Coq Require Import Strings.String.
 
-Inductive map (A : Type) : Type :=
-  | map_nil
-  | map_cons (k : string) (v : A) (m : map A)
-  .
+Local Definition map' (A : Type) := string -> A. (* total map *)
 
-Definition empty {A} := map_nil A.
+Local Definition empty' {A : Type} v : map' A := (fun _ => v).
 
-Fixpoint update {A} (m : map A) k v :=
-  match m with
-  | map_nil _ => map_cons A k v (map_nil A)
-  | map_cons _ k' v' m' =>
-      if eqb k k'
-        then map_cons A k  v  (update m' k v)
-        else map_cons A k' v' (update m' k v)
-  end.
+Local Definition update' {A : Type} (m : map' A) k v :=
+  fun k' => if eqb k k' then v else m k'.
 
-Fixpoint lookup {A} m k : option A :=
-  match m with
-  | map_nil _ => None
-  | map_cons _ k' v m' => if eqb k' k then Some v else lookup m' k
-  end.
+Definition map (A : Type) := map' (option A). (* partial map *)
 
-(* m includes m' *)
-Local Definition includes' {A} (m m' : map A) :=
-  forall k v, lookup m' k = Some v -> lookup m k = Some v.
+Definition empty {A : Type} : map A := empty' None.
 
-Infix "includes" := includes' (at level 50, left associativity).
+Definition update {A : Type} (m : map A) k v :=
+  update' m k (Some v).
 
-Local Definition update' {A} m k v := map_cons A k v m.
+Definition lookup {A : Type} (m : map A) k := m k.
 
-Local Theorem update_equivalence : forall {A} (m : map A) k v id,
-  lookup (update m k v) id = lookup (update' m k v) id.
-Proof.
-  intros *. unfold update', update.
-  induction m as [| k' v' m IH]; trivial.
-  unfold lookup in *.
-  destruct (eqb k k') eqn:E1.
-  - apply eqb_eq in E1. subst. destruct (eqb k' id); trivial.
-  - destruct (eqb k' id) eqn:E2; trivial.
-    apply eqb_eq in E2. subst.
-    destruct (eqb k id) eqn:E3; trivial; discriminate.
-Qed.
+(* Proofs *)
 
-Local Lemma lookup_update_k_eq' : forall {A} (m : map A) k v,
-  lookup (update' m k v) k = Some v.
-Proof.
-  intros. simpl. rewrite String.eqb_refl. reflexivity.
-Qed.
-
-Local Lemma lookup_update_k_neq' : forall {A} (m : map A) k k' v,
-  k' <> k ->
-  lookup (update' m k' v) k = lookup m k.
-Proof.
-  intros * H. simpl. destruct eqb eqn:E; trivial.
-  apply String.eqb_eq in E. contradiction.
-Qed.
-
-Local Lemma update_preserves_inclusion' : forall {A} (m m' : map A) k v,
-  m includes m' ->
-  (update' m k v) includes (update' m' k v).
-Proof.
-  intros *. unfold includes', lookup, update'.
-  destruct m; intros * ? k'; destruct (eqb k k'); eauto.
-Qed.
-
-Local Lemma update_overwrite' : forall {A} (m : map A) k v v',
-  (update' m k v) includes (update' (update' m k v') k v).
-Proof.
-  unfold includes', lookup, update'. intros ? ? ? ? ? k' ?.
-  destruct m; intros H; destruct (eqb k k'); assumption.
-Qed.
-
-Local Lemma update_permutation' : forall {A} (m : map A) k1 k2 v1 v2,
-  k1 <> k2 ->
-  (update' (update' m k1 v1) k2 v2) includes (update' (update' m k2 v2) k1 v1).
-Proof.
-  intros * Hneq. unfold includes'.
-  induction m as [| ? ? ? IH]; intros k' v'.
-  - unfold update', lookup.
-    destruct (eqb k1 k') eqn:E1; trivial.
-    destruct (eqb k2 k') eqn:E2; trivial.
-    apply eqb_eq in E1. apply eqb_eq in E2. subst.
-    contradiction.
-  - specialize (IH k' v').
-    destruct (eqb k1 k') eqn:E1.
-    + apply eqb_eq in E1. subst.
-      destruct (eqb k2 k') eqn:E2.
-      * apply eqb_eq in E2. subst. rewrite 2 lookup_update_k_eq' in *. trivial.
-      * apply eqb_neq in E2.
-        rewrite (lookup_update_k_neq' _ _ _ _ E2).
-        rewrite 2 lookup_update_k_eq' in *.
-        intros H. specialize (IH H).
-        assumption.
-    + apply eqb_neq in E1.
-      rewrite (lookup_update_k_neq' _ _ _ _ E1) in *.
-      destruct (eqb k2 k') eqn:E2.
-      * apply eqb_eq in E2. subst. rewrite 2 lookup_update_k_eq'. trivial.
-      * apply eqb_neq in E2.
-        rewrite 2 (lookup_update_k_neq' _ _ _ _ E2) in *.
-        rewrite (lookup_update_k_neq' _ _ _ _ E1) in *.
-        trivial.
-Qed.
-
-Corollary lookup_update_k_eq : forall {A} (m : map A) k v,
+Lemma lookup_update_keq : forall {A} (m : map A) k v,
   lookup (update m k v) k = Some v.
 Proof.
-  intros. rewrite update_equivalence. auto using lookup_update_k_eq'.
+  intros. unfold lookup, update, update'.
+  rewrite eqb_refl. reflexivity.
 Qed.
 
-Corollary lookup_update_k_neq : forall {A} (m : map A) k k' v,
+Lemma lookup_update_kneq : forall {A} (m : map A) k k' v,
   k' <> k ->
   lookup (update m k' v) k = lookup m k.
 Proof.
-  intros * H. rewrite update_equivalence. auto using lookup_update_k_neq'.
+  intros. unfold lookup, update, update'.
+  destruct eqb eqn:E; trivial.
+  apply eqb_eq in E. contradiction.
 Qed.
 
-Corollary update_preserves_inclusion : forall {A} (m m' : map A) k v,
+(* m includes m' *)
+Definition includes' {A} (m m' : map A) := forall k v,
+  m' k = Some v -> m k = Some v.
+
+Infix "includes" := includes' (at level 50, left associativity).
+
+Lemma update_preserves_inclusion : forall {A} (m m' : map A) k v,
   m includes m' ->
   (update m k v) includes (update m' k v).
 Proof.
-  intros. unfold includes'. intros *.
-  rewrite 2 update_equivalence. apply update_preserves_inclusion'. assumption.
+  unfold includes', update, update'. intros.
+  destruct eqb; auto.
+Qed.
+
+Lemma update_permutation : forall {A} (m : map A) k1 k2 v1 v2,
+  k1 <> k2 ->
+  update (update m k1 v1) k2 v2 includes update (update m k2 v2) k1 v1.
+Proof.
+  unfold includes', update, update'. intros.
+  destruct (eqb k1 k) eqn:E1; destruct (eqb k2 k) eqn:E2; auto.
+  apply eqb_eq in E1, E2. subst. contradiction.
 Qed.
 
 Lemma update_overwrite : forall {A} (m : map A) k v v',
   (update m k v) includes (update (update m k v') k v).
 Proof.
-  unfold includes'. intros ? ? ? ? ? k' ?.
-  rewrite 2 update_equivalence.
-  unfold lookup, update'.
-  destruct m; intros H; destruct (eqb k k') eqn:E; trivial;
-  fold (@lookup A) in H; rewrite update_equivalence in H;
-  unfold lookup, update' in H; rewrite E in H; assumption.
-Qed.
-
-Lemma update_permutation : forall {A} (m : map A) k1 k2 v1 v2,
-  k1 <> k2 ->
-  (update (update m k1 v1) k2 v2) includes (update (update m k2 v2) k1 v1).
-Proof.
-  intros * Hneq. unfold includes'.
-  intros k v. rewrite 2 update_equivalence.
-  generalize dependent v. generalize dependent k.
-  induction m as [| ? ? ? IH]; intros k' v'.
-  - unfold update', lookup.
-    destruct (eqb k1 k') eqn:E1; destruct (eqb k2 k') eqn:E2.
-    + apply eqb_eq in E1, E2. subst. contradiction.
-    + apply eqb_eq in E1. subst.
-      fold (@lookup A). rewrite update_equivalence.
-      unfold update', lookup. rewrite eqb_refl. trivial.
-    + apply eqb_eq in E2. subst.
-      fold (@lookup A). rewrite update_equivalence.
-      unfold update', lookup. rewrite eqb_refl. trivial.
-    + fold (@lookup A). rewrite 2 update_equivalence.
-      unfold update', lookup. rewrite E1, E2. trivial.
-  - specialize (IH k' v').
-    destruct (eqb k1 k') eqn:E1.
-    + apply eqb_eq in E1. subst.
-      destruct (eqb k2 k') eqn:E2.
-      * apply eqb_eq in E2. subst. rewrite 2 lookup_update_k_eq' in *. trivial.
-      * apply eqb_neq in E2.
-        rewrite (lookup_update_k_neq' _ _ _ _ E2).
-        rewrite update_equivalence.
-        rewrite 2 lookup_update_k_eq' in *.
-        trivial.
-    + apply eqb_neq in E1.
-      rewrite (lookup_update_k_neq' _ _ _ _ E1) in *.
-      destruct (eqb k2 k') eqn:E2.
-      * apply eqb_eq in E2. subst.
-        rewrite update_equivalence.
-        rewrite 2 lookup_update_k_eq'.
-        trivial.
-      * apply eqb_neq in E2.
-        rewrite update_equivalence.
-        rewrite 2 (lookup_update_k_neq' _ _ _ _ E2) in *.
-        rewrite (lookup_update_k_neq _ _ _ _ E1) in *.
-        trivial.
+  unfold includes', update, update'. intros.
+  destruct eqb; intros; assumption.
 Qed.
